concurrency/Clight_coreSemantincsForMachines.v
@@ -1,0 +1,39 @@
+Require Import compcert.common.Memory.
+
+Require Import veric.compcert_rmaps.
+Require Import veric.juicy_mem.
+Require Import veric.res_predicates.
+
+(*IM using proof irrelevance!*)
+Require Import ProofIrrelevance.
+
+(* The concurrent machinery*)
+Require Import concurrency.scheduler.
+Require Import concurrency.concurrent_machine.
+Require Import concurrency.semantics.
+Require Import concurrency.juicy_machine. Import Concur.
+Require Import concurrency.dry_machine. Import Concur.
+(*Require Import concurrency.dry_machine_lemmas. *)
+Require Import concurrency.lksize.
+Require Import concurrency.permissions.
+
+(*Semantics*)
+Require Import veric.Clight_core.
+Require Import sepcomp.event_semantics.
+
+Module ClightSEM_core <: Semantics.
+  Definition F: Type := fundef.
+  Definition V: Type := type.
+  Definition G := genv.
+  Definition C := CC_core.
+  Definition getEnv (g:G): Genv.t F V := genv_genv g.
+  (* We might want to define this properly or
+     factor the machines so we don't need events here. *)
+  Parameter CLNC_evsem : @EvSem G C.
+  Parameter CLNC_msem :
+    msem CLNC_evsem = CLNC_memsem.
+  Definition Sem := CLNC_evsem.
+  Parameter step_decay: forall g c m tr c' m',
+      event_semantics.ev_step (Sem) g c m tr c' m' ->
+      decay m m'.
+End ClightSEM_core.
