concurrency/CoreSemantics_sum.v
@@ -1,0 +1,160 @@
+Require Import sepcomp.semantics.
+
+(*
+
+  { initial_core : G -> Values.val -> list Values.val -> option C;
+    at_external : C -> option (AST.external_function * list Values.val);
+    after_external : option Values.val -> C -> option C;
+    halted : C -> option Values.val;
+    corestep : G -> C -> M -> C -> M -> Prop;
+    corestep_not_at_external : forall (ge : G) (m : M) (q : C) (m' : M) (q' : C),
+                               corestep ge q m q' m' -> at_external q = None;
+    corestep_not_halted : forall (ge : G) (m : M) (q : C) (m' : M) (q' : C),
+                          corestep ge q m q' m' -> halted q = None;
+    at_external_halted_excl : forall q : C, at_external q = None \/ halted q = None }
+
+ *)
+
+Inductive state_sum (Cs Ct:Type): Type :=
+| SState (c:Cs)
+| TState (c:Ct).
+
+Definition state_sum_options {Cs Ct:Type} (cso: option Cs): option (state_sum Cs Ct) :=
+  match cso with
+  | Some cs => Some (SState _ _ cs)
+  | _ => None
+  end.
+Definition state_sum_optiont {Cs Ct:Type} (cto: option Ct): option (state_sum Cs Ct) :=
+  match cto with
+  | Some ct => Some (TState _ _ ct)
+  | _ => None
+  end.
+
+Definition lt_op (n: nat) (no:option nat): bool :=
+  match no with
+    | None => true
+    | Some n' => Nat.ltb n n' 
+  end.
+
+Definition initial_core_sum (no:option nat) G (Cs Ct:Type)
+           (sinitial_core : nat -> G -> Values.val -> list Values.val -> option Cs)
+           (tinitial_core : nat -> G -> Values.val -> list Values.val -> option Ct):
+  nat -> G -> Values.val -> list Values.val -> option (state_sum Cs Ct):=
+  fun (n:nat) g val vals =>
+    if lt_op n no
+    then state_sum_options (sinitial_core n g val vals)
+    else state_sum_optiont (tinitial_core n g val vals).
+
+
+Definition sum_func {Cs Ct X:Type} (fs:Cs -> X) (ft:Ct-> X) s:=
+  match s with
+  | SState c => (fs c)
+  | TState c => (ft c)
+  end.
+
+Definition sum_func_option {Cs Ct Cs' Ct':Type} (fs:Cs -> option Cs') (ft:Ct-> option Ct') s:=
+  match s with
+  | SState c => state_sum_options (fs c) 
+  | TState c => state_sum_optiont (ft c) 
+  end.
+
+Definition at_external_sum Cs Ct
+           (sat_external: Cs -> option (AST.external_function * list Values.val))
+           (tat_external: Ct -> option (AST.external_function * list Values.val)):=
+  sum_func sat_external tat_external.
+
+Definition after_external_sum Cs Ct
+           (safter_external: option Values.val -> Cs -> option Cs)
+           (tafter_external: option Values.val -> Ct -> option Ct):=
+  fun vals => sum_func_option (safter_external vals) (tafter_external vals).
+
+Definition halted_sum Cs Ct
+           (shalted: Cs -> option Values.val)
+           (thalted: Ct -> option Values.val):=
+  sum_func shalted thalted.
+
+Inductive corestep_sum {G M Cs Ct}
+          (scorestep: G -> Cs -> M -> Cs -> M -> Prop)
+          (tcorestep: G -> Ct -> M -> Ct -> M -> Prop):
+  G -> state_sum Cs Ct -> M -> state_sum Cs Ct -> M -> Prop:=
+| SCorestep: forall g s m s' m',
+    scorestep g s m s' m' ->
+    corestep_sum scorestep tcorestep g (SState _ _ s) m (SState _ _ s') m'
+| TCorestep: forall g s m s' m',
+    tcorestep g s m s' m' ->
+    corestep_sum scorestep tcorestep g (TState _ _ s) m (TState _ _ s') m'.
+
+Lemma corestep_not_at_external_sum:
+  forall G M Cs Ct
+    (scorestep: G -> Cs -> M -> Cs -> M -> Prop) 
+    (sat_external: Cs -> option (AST.external_function * list Values.val))
+    (scorestep_not_at_external: forall (ge : G) (m : M) (q : Cs) (m' : M) (q' : Cs),
+        scorestep ge q m q' m' -> sat_external q = None)
+    (tcorestep: G -> Ct -> M -> Ct -> M -> Prop)
+    (tat_external: Ct -> option (AST.external_function * list Values.val))
+    (tcorestep_not_at_external: forall (ge : G) (m : M) (q : Ct) (m' : M) (q' : Ct),
+        tcorestep ge q m q' m' -> tat_external q = None),
+  forall (ge : G) (m : M) (q : state_sum Cs Ct) (m' : M) (q' : state_sum Cs Ct),
+    corestep_sum scorestep tcorestep ge q m q' m' ->
+    at_external_sum _ _ sat_external tat_external q = None.
+Proof.
+  intros.
+  inversion H; subst; simpl; eauto.
+Qed.
+
+Lemma corestep_not_halted_sum:
+  forall G M Cs Ct
+    (scorestep: G -> Cs -> M -> Cs -> M -> Prop) 
+    (shalted : Cs -> option Values.val)
+    (scorestep_not_halted: forall (ge : G) (m : M) (q : Cs) (m' : M) (q' : Cs),
+        scorestep ge q m q' m' -> shalted q = None)
+    (tcorestep: G -> Ct -> M -> Ct -> M -> Prop)
+    (thalted : Ct -> option Values.val)
+    (tcorestep_not_halted: forall (ge : G) (m : M) (q : Ct) (m' : M) (q' : Ct),
+        tcorestep ge q m q' m' -> thalted q = None),
+  forall (ge : G) (m : M) (q : state_sum Cs Ct) (m' : M) (q' : state_sum Cs Ct),
+    corestep_sum scorestep tcorestep ge q m q' m' ->
+    halted_sum _ _ shalted thalted q = None.
+Proof.
+  intros.
+  inversion H; subst; simpl; eauto.
+Qed.
+
+Lemma at_external_halted_excl_sum:
+  forall G M Cs Ct
+    (scorestep: G -> Cs -> M -> Cs -> M -> Prop) 
+    (shalted : Cs -> option Values.val)
+    (sat_external: Cs -> option (AST.external_function * list Values.val))
+    (sat_external_halted_excl : forall q : Cs, sat_external q = None \/ shalted q = None)
+    (tcorestep: G -> Ct -> M -> Ct -> M -> Prop)
+    (thalted : Ct -> option Values.val)
+    (tat_external: Ct -> option (AST.external_function * list Values.val))
+    (tat_external_halted_excl : forall q : Ct, tat_external q = None \/ thalted q = None),
+  forall (q : state_sum Cs Ct),
+    at_external_sum _ _ sat_external tat_external q = None \/
+    halted_sum _ _ shalted thalted q = None.
+Proof.
+  intros.
+  destruct q; simpl; auto.
+Qed.
+
+Program Definition CoreSemanticsSum n G M Cs Ct
+        (CSs: CoreSemantics G Cs M )
+        (CSt: CoreSemantics G Ct M ): CoreSemantics G (state_sum Cs Ct) M :=
+  Build_CoreSemantics _ _ _
+    (initial_core_sum n _ _ _ (initial_core CSs) (initial_core CSt))
+    (at_external_sum _ _ (at_external CSs) (at_external CSt))
+    (after_external_sum _ _  (after_external CSs) (after_external CSt))
+    (halted_sum _ _  (halted CSs) (halted CSt))
+    (corestep_sum (corestep CSs) (corestep CSt)) 
+    _ _ _     
+.
+Next Obligation.
+  eapply corestep_not_at_external_sum; eauto; first [apply CSs|apply CSt].
+Qed.
+Next Obligation.
+  eapply corestep_not_halted_sum; eauto; first [apply CSs|apply CSt].
+Qed.
+Next Obligation.
+  eapply at_external_halted_excl_sum; eauto; first [apply CSs|apply CSt].
+Qed.
